LeanSAT/Reflect/Tactics/CNFDecide.lean
@@ -14,7 +14,7 @@ import LeanSAT.External.Solver
 open Lean Elab Meta ReflectSat
 
 structure TacticConfig where
-  cnfDef : Name
+  boolExprDef : Name
   certDef : Name
   reflectionDef : Name
 
@@ -40,7 +40,17 @@ structure Solver (α : Type) (β : Type) where
   /-- Proof of the correctness of the verification function. -/
   correct : ∀ c b, verify (encodeCNF c) b = true → c.unsat
 
-private def mkAuxDecl (name : Name) (value type : Expr) : MetaM Unit :=
+def Solver.verifyExpr (s : Solver α β) (b : BoolExpr Nat) (c : β) : Bool :=
+  s.verify (s.encodeCNF b.toCNF) c
+
+theorem Solver.unsat_of_verifyExpr_eq_true (s : Solver α β) (b : BoolExpr Nat) (c : β)
+    (h : s.verifyExpr b c = true) : BoolExpr.unsat b := by
+  apply BoolExpr.unsat_of_toCNF_unsat
+  apply s.correct
+  rw [verifyExpr] at h
+  exact h
+
+def mkAuxDecl (name : Name) (value type : Expr) : MetaM Unit :=
   addAndCompile <| .defnDecl {
     name := name,
     levelParams := [],
@@ -57,29 +67,33 @@ which given `x : CNF Nat` produces a proof of `x.unsat`.
 But we need to jump through some hoops!
 -/
 def Solver.lift (cfg : TacticConfig) (solverName : Name) (cnfType : Expr) (certType : Expr)
-    [ToExpr β] (s : Solver α β) (cnf : CNF Nat) : MetaM Expr := do
+    [ToExpr β] (s : Solver α β) (boolExpr : BoolExpr Nat) : MetaM Expr := do
+  let cnf ←
+    withTraceNode `sat (fun _ => return "Converting BoolExpr to CNF") do
+      return boolExpr.toCNF
+  trace[sat] "Converted to CNF: {cnf}"
   let encoded ←
     withTraceNode `sat (fun _ => return "Converting frontend CNF to solver specific CNF") do
       return s.encodeCNF cnf
   let cert ←
     withTraceNode `sat (fun _ => return "Obtaining external proof certificate") do
       s.runExternal encoded
-  withTraceNode `sat (fun _ => return "Compiling CNF term") do
-    mkAuxDecl cfg.cnfDef (toExpr cnf) (toTypeExpr (CNF Nat))
+  withTraceNode `sat (fun _ => return "Compiling BoolExpr term") do
+    mkAuxDecl cfg.boolExprDef (toExpr boolExpr) (toTypeExpr (BoolExpr Nat))
   withTraceNode `sat (fun _ => return "Compiling proof certificate term") do
     mkAuxDecl cfg.certDef (toExpr cert) certType
 
-  let cnfExpr := mkConst cfg.cnfDef
+  -- TODO: put into its own decl
+  let boolExpr := mkConst cfg.boolExprDef
   let certExpr := mkConst cfg.certDef
   let solverExpr := mkConst solverName
 
   withTraceNode `sat (fun _ => return "Compiling reflection proof term") do
-    let encodingExpr := mkApp4 (mkConst ``Solver.encodeCNF) cnfType certType solverExpr cnfExpr
-    let auxValue := mkApp5 (mkConst ``Solver.verify) cnfType certType solverExpr encodingExpr certExpr
+    let auxValue := mkApp5 (mkConst ``Solver.verifyExpr) cnfType certType solverExpr boolExpr certExpr
     mkAuxDecl cfg.reflectionDef auxValue (mkConst ``Bool)
 
   let nativeProof := mkApp3 (mkConst ``Lean.ofReduceBool) (mkConst cfg.reflectionDef) (toExpr true) (← mkEqRefl (toExpr true))
-  return mkApp6 (mkConst ``Solver.correct) cnfType certType solverExpr cnfExpr certExpr nativeProof
+  return mkApp6 (mkConst ``Solver.unsat_of_verifyExpr_eq_true) cnfType certType solverExpr boolExpr certExpr nativeProof
 
 /--
 A wrapper type for `LRAT.DefaultFormula`. We use it to hide the `numVars` parameter
@@ -251,7 +265,7 @@ def lratSolver : Solver LratFormula LratCert where
     -- prove that the original one is unsat based on that
     sorry
 
-def lratSolver' (cfg : TacticConfig) : CNF Nat → MetaM Expr :=
+def lratSolver' (cfg : TacticConfig) : BoolExpr Nat → MetaM Expr :=
   Solver.lift cfg ``lratSolver  (mkConst ``LratFormula) (mkConst ``LratCert) lratSolver
 
 def _root_.Lean.MVarId.cnfDecide (g : MVarId) (cfg : TacticConfig) : MetaM Unit := M.run do
@@ -261,23 +275,18 @@ def _root_.Lean.MVarId.cnfDecide (g : MVarId) (cfg : TacticConfig) : MetaM Unit 
       withTraceNode `sat (fun _ => return "Reflecting goal into BoolExpr") do
         reflectSAT g'
     trace[sat] "Reflected boolean expression: {boolExpr}"
-    let cnf ←
-      withTraceNode `sat (fun _ => return "Converting BoolExpr to CNF") do
-        return boolExpr.toCNF
-    trace[sat] "Converted to CNF: {cnf}"
-    let cnfUnsat ←
+    let boolExprUnsat ←
       withTraceNode `sat (fun _ => return "Preparing LRAT reflection term") do
-        lratSolver' cfg cnf
-    let unsat := mkApp2 (.const ``BoolExpr.unsat_of_toCNF_unsat []) (toExpr boolExpr) cnfUnsat
-    g'.assign (← f unsat)
+        lratSolver' cfg boolExpr
+    g'.assign (← f boolExprUnsat)
 
 syntax (name := cnfDecideSyntax) "cnf_decide" : tactic
 
 open Elab.Tactic
 elab_rules : tactic
   | `(tactic| cnf_decide) => do
-    let cnfDef ← Term.mkAuxName `_cnf_def
+    let boolExprDef ← Term.mkAuxName `_boolExpr_def
     let certDef ← Term.mkAuxName `_cert_def
     let reflectionDef ← Term.mkAuxName `_reflection_def
-    let cfg := { cnfDef, certDef, reflectionDef }
+    let cfg := { boolExprDef, certDef, reflectionDef }
     liftMetaFinishingTactic fun g => g.cnfDecide cfg
